finished full implemetations of lock-coupling and giveup for linked-list and bst

concurrency/Modular/implementations/bst_giveup.c
@@ -1,0 +1,55 @@
+#include "bst_giveup.h"
+
+void insertOp_giveup(node_t* p, int x, void* value, Status status){
+    node_t* p1 = (struct node_t*)surely_malloc(sizeof (node_t));
+    node_t* p2 = (struct node_t*)surely_malloc(sizeof (node_t));
+    p1->t = NULL;
+    p2->t = NULL;
+
+    lock_t* l1 = (lock_t*)surely_malloc(sizeof(lock_t));
+    makelock(l1);
+    p1->lock = l1;
+    release(l1);
+
+    lock_t* l2 = (lock_t*)surely_malloc(sizeof(lock_t));
+    makelock(l2);
+    p2->lock = l2;
+    release(l2);
+
+    DList dlist; 
+    dlist.size = 2; // For BST 
+    dlist.list = (void**)surely_malloc(dlist.size * sizeof(node_t));
+    dlist.list[0] = p1;
+    dlist.list[1] = p2;
+
+    insertOp(&p->t, x, value, status, &dlist);
+
+    ((node_t*)dlist.list[0])->min = p->min;
+    ((node_t*)dlist.list[0])->max = x;
+    ((node_t*)dlist.list[1])->min = x;
+    ((node_t*)dlist.list[1])->max = p->max;
+} 
+
+void printDS_giveup(void **t){
+    printf("For BST - GIVEUP\n");
+    struct node_t* tgt;
+    tgt = *t;
+
+    if (tgt == NULL) {
+        return;
+    }
+    stack s;
+    initStack(&s);
+    node_t * current = tgt;
+
+    while (current->t != NULL || !isEmpty(&s)) {
+        while (current->t != NULL) {
+            push(&s, current);
+            current = (node_t *)getLeftChild(current->t);
+        }
+
+        current = pop(&s);
+        printKey(current->t);
+        current = (node_t *)getRightChild(current->t);
+    }
+}
