concurrency/Modular/implementations/giveup_template.c
@@ -1,0 +1,163 @@
+//
+//  give_up_template.c
+//  BST
+//
+//  Created by Duc Than Nguyen on 5/29/23.
+//
+
+#include "giveup_template.h"
+
+int inRange(node_t *p, int x){
+    if (x > p->min && x < p->max)
+        return 1;
+    else
+        return 0;
+}
+//FOUND == 0, NOTFOUND = 1, NULLNEXT = 2
+Status traverse(pn *pn, int x) {
+    Status status = 2; //NULLNEXT
+    void *p = (pn->n);
+    for( ; ; ){
+        acquire(pn->n->lock);
+        pn->p = pn->n;
+        if (inRange (pn->p, x) == 1){
+            if (pn->p->t == NULL){
+                status = NULLNEXT;
+                break;
+            }
+            else{
+                status = findNext(pn->p->t, (void**)&pn->n, x);
+                if (status == FOUND){
+                    status = FOUND;
+                    break;
+                }
+                else if (status == NOTFOUND){
+                    status = NOTFOUND;
+                    break;
+                }
+                else{
+                    release(pn->p->lock);
+                }
+            }
+        }
+        else{
+            release(pn->p->lock);
+            pn->n = p;
+        }
+            
+    }
+    return status;
+}
+
+/*
+void insertOp_list(node_t* p, int x, void* value, Status status){
+    struct node_t* pl; 
+    pl = (struct node_t*)surely_malloc(sizeof (node_t));
+    if (status == NULLNEXT) {
+        pl->t = NULL;
+        lock_t* l = (lock_t*)surely_malloc(sizeof(lock_t));
+        makelock(l);
+        pl->lock = l;
+        release(l); 
+
+        insertOp_llist(&p->t, x, value, status, pl);
+        pl->max = INT_MAX;
+        pl->min = x;
+    }
+    else{
+        lock_t* l = (lock_t*)surely_malloc(sizeof(lock_t));
+        makelock(l);
+        pl->lock = l;
+        release(l);
+        pl->t = p->t;
+        pl->max = p->max; 
+        pl->min = x; 
+        insertOp_llist(&(p->t), x, value, status, pl);
+    }
+} 
+*/
+/*
+void insertOp_list(node_t* p, int x, void* value, Status status){
+    DList dlist; 
+    dlist.size = 1; // For Linked-list 
+    dlist.list = (void**)surely_malloc(dlist.size * sizeof(node_t));
+    dlist.list[0] = (struct node_t*)surely_malloc(sizeof (node_t));
+    if (status == NULLNEXT) {
+        ((node_t*)dlist.list[0])->t = NULL;
+        lock_t* l = (lock_t*)surely_malloc(sizeof(lock_t));
+        makelock(l);
+        ((node_t*)dlist.list[0])->lock = l;
+        release(l);
+        insertOp_llist(&p->t, x, value, status, &dlist);
+        ((node_t*)dlist.list[0])->min = x;
+        ((node_t*)dlist.list[0])->max = INT_MAX;
+    }
+    else{
+        lock_t* l = (lock_t*)surely_malloc(sizeof(lock_t));
+        makelock(l);
+        ((node_t*)dlist.list[0])->lock = l;
+        release(l);
+        ((node_t*)dlist.list[0])->t = p->t;
+        ((node_t*)dlist.list[0])->max = p->max; 
+        ((node_t*)dlist.list[0])->min = x;
+        insertOp_llist(&(p->t), x, value, status, &dlist);
+    }
+}
+*/
+void insertOp_helper(node_t *p, int x, void* value, Status status){
+    insertOp_giveup(p, x, value, status);
+    //insertOp_list(p, x, value, status);
+}
+
+node_t * treebox_helper(node_t *newt){
+    newt = (node_t *) surely_malloc(sizeof(node_t));
+    lock_t *l = (lock_t *) surely_malloc(sizeof(lock_t));
+    makelock(l);
+    newt->lock = l;
+    newt->t = NULL;
+    newt->min = INT_MIN;
+    newt->max = INT_MAX;
+    release(l);
+    return newt;
+}
+
+lock_t* getLock(node_t *p){
+    return p->lock;
+}
+
+void changeValue_helper(node_t *p, void * value){
+    changeValue(p->t, value);
+}
+
+void *getValue_helper(node_t* p){
+    return getValue(p->t);
+}
+
+//for BST
+
+void printDS_helper (void **t){
+    printDS_giveup(t);
+}
+
+
+/*
+void printDS_helper (void **t){
+    struct node_t* tgt;
+    tgt = *t;
+
+    if (tgt == NULL) {
+        return;
+    }
+    stack s;
+    initStack(&s);
+    node_t * current = tgt;
+    while (current->t != NULL) {
+        push(&s, current);
+        current = (node_t *)getNext(current->t);
+    }
+    while (!isEmpty(&s)){   
+        current = pop(&s);
+        printKey(current->t);
+    }
+}
+*/
