concurrency/Modular/implementations/template.c
@@ -1,0 +1,62 @@
+//
+//  template.c
+//  BST
+//
+//  Created by Duc Than Nguyen on 6/22/23.
+//
+
+#include <stdio.h>
+#include <limits.h>
+#include <stdlib.h>
+#include "threads.h"
+#include "template.h"
+
+void insert (treebox t, int x, void *value) {
+    struct pn *pn = (struct pn *) surely_malloc (sizeof *pn);
+    pn->n = *t;
+    Status status = traverse(pn, x);
+    if (status == 0){
+        changeValue_helper(pn->p, value);
+    }
+    else
+    {
+        insertOp_helper(pn->p, x, value, status);
+    }
+    release(getLock(pn->n));
+    free(pn);
+}
+
+
+void *lookup (treebox t, int x) {
+    struct pn *pn = (struct pn *) surely_malloc (sizeof *pn);
+    void *v;
+    pn->n = *t;
+    Status status = traverse(pn, x);
+    if (status == FOUND){
+        v = getValue_helper(pn->p);
+    }
+    else
+    {
+        v = NULL;
+    }
+    release(getLock(pn->n));
+    free(pn);
+    return v;
+}
+
+
+treebox treebox_new(void) {
+    treebox p = (treebox) surely_malloc(sizeof (*p));
+    node_t *newt;
+    //*p = newt;
+    *p = treebox_helper(newt);
+    return p;
+}
+
+/*
+void treebox_free(treebox b) {
+    struct node_t *t = *b;
+    freeDS(t);
+    free(b);
+}
+*/
