concurrency/Modular/giveup_proofs.v
@@ -1,10 +1,11 @@
 Require Import VST.concurrency.conclib.
 Require Import VST.floyd.proofauto.
 Require Import VST.atomics.general_locks.
-Require Import bst.giveup_template. (* giveup_template.c *)
+Require Import bst.giveup_template.
 Require Import bst.puretree.
 Require Import bst.data_struct.     
-Require Import bst.giveup_lib.
+Require Import bst.giveup_lib. 
+Require Import bst.giveup_specs.
 Require Import VST.atomics.verif_lock_atomic.
 Require Import VST.floyd.library.
 
@@ -12,132 +13,9 @@ Require Import VST.floyd.library.
 Definition Vprog : varspecs.  mk_varspecs prog. Defined.
 
 
-#[global] Instance gmap_inhabited V : Inhabitant (gmap key V).
-Proof. unfold Inhabitant; apply empty. Defined.
-
-#[global] Instance number_inhabited: Inhabitant number.
-Proof. unfold Inhabitant; apply Pos_Infinity. Defined.
-
-Definition surely_malloc_spec :=
-  DECLARE _surely_malloc
-   WITH t: type, gv: globals
-   PRE [ size_t ]
-       PROP (and (Z.le 0 (sizeof t)) (Z.lt (sizeof t) Int.max_unsigned);
-                complete_legal_cosu_type t = true;
-                natural_aligned natural_alignment t = true)
-       PARAMS (Vptrofs (Ptrofs.repr (sizeof t))) GLOBALS (gv)
-       SEP (mem_mgr gv)
-    POST [ tptr tvoid ]
-    EX p: _,
-       PROP ()
-       RETURN (p)
-       SEP (mem_mgr gv; malloc_token Ews t p * data_at_ Ews t p).
-
-
-Lemma test (pt: enum * (val * (share * (gname * node_info )))) (pt1 : node_info): True.
-  Proof.
-    Check (((pt.2.2.2).2).1).2.
-    Check pt.2.2.1. (*share *)
-    Check ((((pt.2.2.2).2).1).1).2.
-    Check ((pt1.1).1).2.
-    Check (pt.2.2.2).2.
-    Check (pt1.1).2.
-    Check ((((pt.2.2.2).2).1).1).1.
-    Check pt.2.2.2.2.
-    Check ((pt1.1).1).1.
-    Check (pt.2.2.2).2.
-    Admitted.
-
-Definition post_traverse (b: val) x (g: gname) (e: enum) (p: val) (sh: share) (g_in: gname) (n: node_info):=
-  !!( key_in_range x (n.1).2 = true ∧
-      repable_signed (number2Z (n.1).2.1) /\ repable_signed (number2Z (n.1).2.2) /\
-      is_pointer_or_null (((n.1).1).2) /\
-      (if Val.eq (enums e) (enums NN)
-       then n.2 = Some None /\ ((n.1).1).1 = nullval
-                          else ((n.1).1).1 <> nullval)
-                        (* (match (pt.1 : enum) with
-                         | NN => pt.2.2.2.2.2 = Some None /\ ((((pt.2.2.2).2).1).1).1 = nullval
-                         | NF | F =>  ((((pt.2.2.2).2).1).1).1 <> nullval
-                        (* | NF => ((((pt.2.2.2).2).1).1).1 <> nullval *)
-                          end) *)  ) && seplog.emp * 
-  data_at Ews t_struct_pn (p, p) b * in_tree g g_in p ((n.1).1).2 * node_lock_inv_pred g p g_in n.
-
-(*
-Program Definition traverse_spec :=
-  DECLARE _traverse
-          ATOMIC TYPE (rmaps.ConstType
-                       (val * val * val * Z  * val * globals * gname * gname))
-          OBJ M INVS ∅
-  WITH b, n, lock, x, v, gv, g, g_root
-  PRE [ tptr t_struct_pn, tint]
-  PROP (and (Z.le (Int.min_signed) x) (Z.le x (Int.max_signed)); is_pointer_or_null v)
-  PARAMS (b; Vint (Int.repr x)) GLOBALS (gv)
-  SEP  (mem_mgr gv; 
-        in_tree g g_root n lock;
-        !!(is_pointer_or_null lock /\ is_pointer_or_null n) && seplog.emp;
-        EX (p: val), data_at Ews (t_struct_pn) (p, n) b ) | (CSS g g_root M)
-  POST [ tint ]
-  EX  pt: enum * (val * (share * (gname * node_info ))) %type,
-  PROP ()
-  LOCAL (temp ret_temp (enums pt.1))
-  SEP (mem_mgr gv; !!( key_in_range x (((pt.2.2.2).2).1).2 = true ∧
-                         repable_signed (number2Z (((pt.2.2.2).2).1).2.1) ∧
-                         repable_signed (number2Z (((pt.2.2.2).2).1).2.2) /\
-                         is_pointer_or_null ((((pt.2.2.2).2).1).1).2
-                       /\ (if Val.eq (enums pt.1) (enums NN) then
-                            pt.2.2.2.2.2 = Some None /\ ((((pt.2.2.2).2).1).1).1 = nullval
-                          else ((((pt.2.2.2).2).1).1).1 <> nullval)
-                        (* (match (pt.1 : enum) with
-                         | NN => pt.2.2.2.2.2 = Some None /\ ((((pt.2.2.2).2).1).1).1 = nullval
-                         | NF | F =>  ((((pt.2.2.2).2).1).1).1 <> nullval
-                        (* | NF => ((((pt.2.2.2).2).1).1).1 <> nullval *)
-                          end) *)  ) && seplog.emp; 
-        data_at Ews t_struct_pn (pt.2.1, pt.2.1) b;
-        in_tree g pt.2.2.2.1 pt.2.1 ((((pt.2.2.2).2).1).1).2;
-       node_lock_inv_pred g pt.2.1 pt.2.2.2.1 (pt.2.2.2).2)| (CSS g g_root M).
-*)
-
-Program Definition traverse_spec :=
-  DECLARE _traverse
-          ATOMIC TYPE (rmaps.ConstType
-                       (val * val * val * Z  * val * globals * gname * gname))
-          OBJ M INVS ∅
-  WITH b, n, lock, x, v, gv, g, g_root
-  PRE [ tptr t_struct_pn, tint]
-  PROP (and (Z.le (Int.min_signed) x) (Z.le x (Int.max_signed)); is_pointer_or_null v)
-  PARAMS (b; Vint (Int.repr x)) GLOBALS (gv)
-  SEP  (mem_mgr gv; 
-        in_tree g g_root n lock;
-        !!(is_pointer_or_null lock /\ is_pointer_or_null n) && seplog.emp;
-        EX (p: val), data_at Ews (t_struct_pn) (p, n) b ) | (CSS g g_root M)
-  POST [ tint ]
-  EX  pt: enum * (val * (share * (gname * node_info ))) %type,
-  PROP ()
-  LOCAL (temp ret_temp (enums pt.1))
-  SEP (mem_mgr gv; post_traverse b x g pt.1 pt.2.1 pt.2.2.1 pt.2.2.2.1 (pt.2.2.2).2)| (CSS g g_root M).
-
-
-(* t_struct_node represents for the generic-struct rather specific-data-structure *)
-(* Spec of inrange function *)
-Definition inRange_spec :=
-  DECLARE _inRange
-    WITH x: Z, p: val, min: Z, max : Z, sh: share, gv: globals
-  PRE [ tptr t_struct_node, tint]
-          PROP (writable_share sh; repable_signed min; repable_signed max; repable_signed x)
-          PARAMS (p; Vint (Int.repr x)) GLOBALS (gv)
-          SEP (
-              field_at sh (t_struct_node) [StructField _min] (Vint (Int.repr min)) p;
-              field_at sh (t_struct_node) [StructField _max] (Vint (Int.repr max)) p)
-  POST [ tint ]
-  EX (succ: bool),
-         PROP (match succ with
-               | true => (and (Z.lt min x) (Z.lt x max))
-               | false => (or (Z.le x min) (Z.le max x))
-               end)
-        LOCAL (temp ret_temp (Vint (if succ then Int.one else Int.zero)))
-        SEP (
-             field_at sh (t_struct_node) [StructField _min] (Vint (Int.repr min)) p;
-              field_at sh (t_struct_node) [StructField _max] (Vint (Int.repr max)) p).
+Definition Gprog : funspecs :=
+    ltac:(with_library prog [acquire_spec; release_spec; makelock_spec; findnext_spec; 
+                             inRange_spec; traverse_spec; insertOp_bst_spec; surely_malloc_spec ]).
 
 Lemma node_rep_saturate_local r p g g_current:
   node_rep p g g_current r |-- !! is_pointer_or_null p.
@@ -154,59 +32,15 @@ Proof.
 Qed.
 Global Hint Resolve node_rep_valid_pointer : valid_pointer.
 
-(*
-(* Spec of findnext function *)
-(* FOUND = 0, NOTFOUND = 1, NULLNEXT = 2 (NULLNEXT = NULL || NEXT ) *)
-Definition findnext_spec :=
-  DECLARE _findNext
-  WITH x: Z, p: val, n: val, n_pt : val, r : node_info, g: gname, sh: share, gv: globals
-  PRE [ tptr tvoid, tptr (tptr tvoid), tint ]
-          PROP (writable_share sh(*; is_pointer_or_null pa; is_pointer_or_null pb*) )
-          PARAMS (p; n; Vint (Int.repr x)) GLOBALS (gv)
-          SEP ((* data_at sh (t_struct_tree_t) (p, n) b *)
-            node_rep_R r.1.1.1 r.1.2 r.2 g ;
-               field_at sh (t_struct_node) [StructField _t] r.1.1.1 p;
-               data_at sh (tptr t_struct_node) n_pt n)
-  POST [ tint ]
-  EX (stt: enum), EX (n' next : val),
-         PROP (match stt with
-               | F | NF => (n' = p)
-               | NN => (n' = next)
-               end)
-        LOCAL (temp ret_temp (enums stt))
-        SEP (match stt with
-               | F | NF => data_at sh (tptr t_struct_node) n_pt n
-               | NN => !!(n' ∈ extract_node_pn r) && data_at sh (tptr t_struct_node) next n
-             end *
-               node_rep_R r.1.1.1 r.1.2 r.2 g *
-               field_at sh (t_struct_node) [StructField _t] r.1.1.1 p).
-*)
+Lemma node_rep_R_saturate_local: forall pt r g_info g,
+  node_rep_R pt r g_info g |-- !! is_pointer_or_null pt.
+Proof. intros; by pose proof (node_rep_R_pointer_null). Qed.
+Global Hint Resolve node_rep_R_saturate_local: saturate_local.
 
-(* Spec of findnext function *)
-(* FOUND = 0, NOTFOUND = 1, NULLNEXT = 2 (NULLNEXT = NULL || NEXT ) *)
-Definition findnext_spec :=
-  DECLARE _findNext
-  WITH x: Z, p: val, n: val, n_pt : val, r: node_info,
-                g: gname, sh: share, gv: globals
-  PRE [ tptr t_struct_nodeds, tptr (tptr tvoid), tint ]
-          PROP (writable_share sh(*; is_pointer_or_null pa; is_pointer_or_null pb*) )
-          PARAMS (p; n; Vint (Int.repr x)) GLOBALS (gv)
-          SEP (node_rep_R r.1.1.1 r.1.2 r.2 g * (!!(p = r.1.1.1) && seplog.emp) *
-               (* field_at sh (t_struct_tree) [StructField _t] r.1.1.1 p; *)
-               
-               data_at sh (tptr t_struct_node) n_pt n)
-  POST [ tint ]
-  EX (stt: enum), EX (n' next : val),
-         PROP (match stt with
-               | F | NF => (n' = p)
-               | NN => (n' = next)
-               end)
-        LOCAL (temp ret_temp (enums stt))
-        SEP (match stt with
-               | F | NF => data_at sh (tptr t_struct_node) n_pt n
-               | NN => !!(n' ∈ extract_node_pn r) && data_at sh (tptr t_struct_node) next n
-             end *
-               node_rep_R r.1.1.1 r.1.2 r.2 g) .
+Lemma node_rep_R_valid_pointer: forall t tp g_children g,
+  node_rep_R tp t g_children g |-- valid_pointer tp.
+Proof. intros; by pose proof (node_rep_R_valid_pointer). Qed.
+Global Hint Resolve node_rep_R_valid_pointer : valid_pointer.
 
 (* Proving inrange spec *)
 Lemma body_inrange: semax_body Vprog Gprog f_inRange inRange_spec.
@@ -239,6 +73,32 @@ Proof.
       Exists false. entailer !.
 Qed.
 
+Lemma insertOp_bst: semax_body Vprog Gprog f_insertOp_bst insertOp_bst_spec.
+Proof.
+  start_function.
+  forward_call (t_struct_node, gv).
+  Intros p1.
+  forward_call (t_struct_node, gv).
+  Intros p2.
+  forward.
+  assert_PROP (field_compatible t_struct_node [] p1) by entailer!.
+  assert_PROP (field_compatible t_struct_node [] p2) by entailer!.
+  forward. 
+  forward_call (gv).
+  Intros lock1.
+  forward.
+  sep_apply atomic_int_isptr.
+  Intros.
+  forward_call release_nonatomic (lock1).
+  forward_call (gv).
+  Intros lock2.
+  forward.
+  Intros.
+  forward_call release_nonatomic (lock2).
+  (* make lock invariant *)
+  Admitted.
+
+
 (* traverse invariants *)
 Definition traverse_inv (b: val) (n pnN': val) (sh: share)
                         (x : Z) (v: val) (g_root: gname) (lock: val) gv
@@ -264,76 +124,6 @@ Definition traverse_inv_2 (b p: val) (sh : share) (x : Z) (g_root g_in g: gname)
   (* node_lock_inv_pred_1 g p g_in r x * *) (* modify it later*)
   (!!(repable_signed (number2Z r.1.2.1) ∧
       repable_signed (number2Z r.1.2.2) /\ is_pointer_or_null r.1.1.2) && seplog.emp).
-
-Definition insertOp_bst_spec :=
-  DECLARE _insertOp_bst
-    WITH x: Z, stt: Z,  v: val, p: val, tp: val, min: Z, max: Z, gv: globals
-  PRE [ tptr t_struct_node, tint, tptr tvoid, tint ]
-  PROP (repable_signed min; repable_signed max; repable_signed x;
-        is_pointer_or_null v )
-  PARAMS (p; Vint (Int.repr x); v; Vint (Int.repr stt))
-  GLOBALS (gv)
-  SEP (mem_mgr gv;
-       field_at Ews t_struct_node (DOT _t) tp p;
-       field_at Ews t_struct_node (DOT _min) (vint min) p;
-       field_at Ews t_struct_node (DOT _max) (vint max) p)
-  POST[ tvoid ]
-  EX (pnt : val) (pnl: list val) (lkl: list val),
-  PROP (pnt <> nullval)
-  LOCAL ()
-  SEP (mem_mgr gv;
-       (* data_at sh t_struct_pn (p, p) b; *)
-       field_at Ews t_struct_node (DOT _t) pnt p;
-       malloc_token Ews t_struct_node pnt;
-       iter_sepcon (fun pn => malloc_token Ews t_struct_node pn) pnl;
-       iter_sepcon (fun lk => atomic_int_at Ews (vint 0) lk) lkl;
-(*
-       data_at Ews t_struct_tree (vint x, (v, (p1', p2'))) pnt;
-       data_at Ews t_struct_tree_t (Vlong (Int64.repr 0), (lock2, (vint x, vint max))) p2';
-       data_at Ews t_struct_tree_t (Vlong (Int64.repr 0), (lock1, (vint min, vint x))) p1';
-*)
-       field_at Ews t_struct_node (DOT _min) (vint min) p;
-       field_at Ews t_struct_node (DOT _max) (vint max) p).
-
-Definition Gprog : funspecs :=
-    ltac:(with_library prog [acquire_spec; release_spec; makelock_spec; findnext_spec; 
-                             inRange_spec; traverse_spec; insertOp_bst_spec; surely_malloc_spec ]).
-
-Lemma node_rep_R_saturate_local: forall pt r g_info g,
-  node_rep_R pt r g_info g |-- !! is_pointer_or_null pt.
-Proof. intros; by pose proof (node_rep_R_pointer_null). Qed.
-Global Hint Resolve node_rep_R_saturate_local: saturate_local.
-
-Lemma node_rep_R_valid_pointer: forall t tp g_children g,
-  node_rep_R tp t g_children g |-- valid_pointer tp.
-Proof. intros; by pose proof (node_rep_R_valid_pointer). Qed.
-Global Hint Resolve node_rep_R_valid_pointer : valid_pointer.
-
-
-Lemma insertOp_bst: semax_body Vprog Gprog f_insertOp_bst insertOp_bst_spec.
-Proof.
-  start_function.
-  forward_call (t_struct_node, gv).
-  Intros p1.
-  forward_call (t_struct_node, gv).
-  Intros p2.
-  forward.
-  assert_PROP (field_compatible t_struct_node [] p1) by entailer!.
-  assert_PROP (field_compatible t_struct_node [] p2) by entailer!.
-  forward. 
-  forward_call (gv).
-  Intros lock1.
-  forward.
-  sep_apply atomic_int_isptr.
-  Intros.
-  forward_call release_nonatomic (lock1).
-  forward_call (gv).
-  Intros lock2.
-  forward.
-  Intros.
-  forward_call release_nonatomic (lock2).
-  (* make lock invariant *)
-  Admitted.
 
 
 (* PROVING traverse spec *)
