concurrency/Modular/bst_inst.v
@@ -3,7 +3,7 @@ Require Import VST.floyd.proofauto.
 Require Import VST.atomics.general_locks.
 Require Import bst.puretree.
 Require Import bst.bst.
-Require Import bst.dataStruct.
+Require Import bst.data_struct.
 Require Import VST.atomics.verif_lock_atomic.
 Require Import VST.floyd.library.
 
@@ -14,20 +14,36 @@ Definition Vprog : varspecs.  mk_varspecs prog. Defined.
 Definition t_struct_tree := Tstruct _node noattr.
 
 (* struct tree_t {node *t; lock_t *lock; int min; int max; } tree_t; *)
-Definition t_struct_tree_t := Tstruct _tree_t noattr.
+(* Definition t_struct_tree_t := Tstruct _tree_t noattr. *)
 
 (* node_rep_R r.1.1.1 r.1.2 r.2 g, and r is type of node_info *)
-#[local]Instance my_specific_tree_rep : NodeRep := {
-  node_rep_R := fun tp r g_info g =>
-    EX (ga gb : gname), EX (x : Z), EX (v pa pb : val), EX (locka lockb : val),
+
+
+#[local] Obligation Tactic := idtac.
+
+#[local] Program Instance my_specific_tree_rep : NodeRep := {
+  node_rep_R := fun (tp : val) (r : range) (g_info : option (option ghost_info)) g =>
+  if eq_dec tp nullval
+  then !!(g_info = Some None) && seplog.emp
+  else
+  (EX (x : Z), EX (v pa pb : val),
       !!(g_info = Some (Some (x, v, [pa; pb])) /\ and (Z.le Int.min_signed x) (Z.le x Int.max_signed) /\
-       is_pointer_or_null pa /\ is_pointer_or_null locka /\
-       is_pointer_or_null pb /\ is_pointer_or_null lockb /\
+       is_pointer_or_null pa /\ is_pointer_or_null pb /\
           (tc_val (tptr Tvoid) v) /\ key_in_range x r = true) &&
        data_at Ews t_struct_tree ((Vint (Int.repr x)), (v, (pa, pb))) tp * 
-       malloc_token Ews t_struct_tree tp *
-       in_tree g ga pa locka * in_tree g gb pb lockb
-}.
+       malloc_token Ews t_struct_tree tp)}.
+
+(* ; node_rep_R_valid_pointer }. *)
+Next Obligation.
+  simpl.
+  intros tp r g_info g.
+  destruct (EqDec_val tp nullval); [ | Intros x v pa pb]; entailer !.
+Defined.
+Next Obligation.
+  simpl.
+  intros tp r g_info g.
+  destruct (EqDec_val tp nullval); [ | Intros x v pa pb]; entailer !.
+Defined.
 
 Definition extract_node_pn (node: node_info) : list val :=
   match node.2 with
@@ -39,13 +55,15 @@ Definition extract_node_pn (node: node_info) : list val :=
 (* FOUND = 0, NOTFOUND = 1, NULLNEXT = 2 (NULLNEXT = NULL || NEXT ) *)
 Definition findnext_spec :=
   DECLARE _findNext
-  WITH x: Z, p: val, n: val, n_pt : val, tp: val, r : node_info, g: gname, sh: share, gv: globals
-  PRE [ tptr tvoid, tptr (tptr tvoid), tint ]
+  WITH x: Z, p: val, n: val, n_pt : val, r: node_info,
+                g: gname, sh: share, gv: globals
+  PRE [ tptr t_struct_tree, tptr (tptr tvoid), tint ]
           PROP (writable_share sh(*; is_pointer_or_null pa; is_pointer_or_null pb*) )
           PARAMS (p; n; Vint (Int.repr x)) GLOBALS (gv)
-          SEP (node_rep_R r.1.1.1 r.1.2 r.2 g ;
-               field_at sh (t_struct_tree_t) [StructField _t] r.1.1.1 p;
-               data_at sh (tptr t_struct_tree_t) n_pt n)
+          SEP (node_rep_R r.1.1.1 r.1.2 r.2 g * (!!(p = r.1.1.1 /\ p <> nullval) && seplog.emp) *
+               (* field_at sh (t_struct_tree) [StructField _t] r.1.1.1 p; *)
+               
+               data_at sh (tptr tvoid) n_pt n)
   POST [ tint ]
   EX (stt: enum), EX (n' next : val),
          PROP (match stt with
@@ -54,31 +72,34 @@ Definition findnext_spec :=
                end)
         LOCAL (temp ret_temp (enums stt))
         SEP (match stt with
-               | F | NF => data_at sh (tptr t_struct_tree_t) n_pt n
-               | NN => !!(n' ∈ extract_node_pn r) && data_at sh (tptr t_struct_tree_t) next n
+               | F | NF => data_at sh (tptr tvoid) n_pt n
+               | NN => !!(n' ∈ extract_node_pn r) && data_at sh (tptr tvoid) next n
              end *
-               node_rep_R r.1.1.1 r.1.2 r.2 g *
-               field_at sh (t_struct_tree_t) [StructField _t] r.1.1.1 p).
+               node_rep_R r.1.1.1 r.1.2 r.2 g) .
 
 
 Lemma findNext: semax_body Vprog Gprog f_findNext findnext_spec.
 Proof.
   start_function.
-  (* int y = pn->p->t->key *)
-  forward.
   unfold node_rep_R.
   unfold my_specific_tree_rep.
-  Intros ga gb x0 v0 pa pb locka lockb.
-  repeat forward.
+  Intros.
+  subst.
+  rewrite -> if_false; eauto.
+  Intros x0 v0 pa pb.
+  forward.
   forward_if. (* if (_x < _y) *)
   - (* pn->n = pn->p->t->left *)
-    repeat forward.
+    forward. forward. forward.
     Exists NN pa pa.
     entailer !.
     unfold extract_node_pn.
     rewrite H.
     apply elem_of_list_here.
-    Exists ga gb x0 v0 pa pb locka lockb.
+    rewrite H.
+    simpl.
+    rewrite -> if_false; eauto.
+    Exists x0 v0 pa pb.
     entailer !.
   - forward_if.
     (* pn->n = pn->p->t->right *)
@@ -88,21 +109,21 @@ Proof.
     unfold extract_node_pn.
     rewrite H.
     assert([pa ; pb] = [pa] ++ [pb]); auto.
-    rewrite H13.
+    rewrite H12.
     rewrite elem_of_app. right.
     apply elem_of_list_here.
-    Exists ga gb x0 v0 pa pb locka lockb.
+    simpl.
+    rewrite -> if_false; eauto.
+    Exists x0 v0 pa pb.
     entailer !.
     forward.
-    Exists F p n_pt.
+    Exists F r.1.1.1  n_pt.
     entailer !.
-    Intros.
-    Exists ga gb x0 v0 pa pb locka lockb.
+    simpl.
+    rewrite -> if_false; eauto.
+    Exists x0 v0 pa pb.
     entailer !.
 Qed.
-
-Check enums.
-Check tint.
 
 Definition surely_malloc_spec :=
   DECLARE _surely_malloc
@@ -119,38 +140,25 @@ Definition surely_malloc_spec :=
        RETURN (p)
        SEP (mem_mgr gv; malloc_token Ews t p * data_at_ Ews t p).
 
-Check iter_sepcon (fun p => malloc_token Ews t_struct_tree_t p) [_; _].
+Check iter_sepcon (fun p => malloc_token Ews _ p) [_; _].
 
 Definition insertOp_spec :=
   DECLARE _insertOp
-    WITH b: val, sh: share, x: Z, stt: Z,  v: val, p: val, tp: val, min: Z, max: Z, gv: globals
-  PRE [ tptr tvoid, tint, tptr tvoid, tint ]
-  PROP (writable_share sh; repable_signed min; repable_signed max; repable_signed x;
-        is_pointer_or_null v )
-  PARAMS (p; Vint (Int.repr x); v; Vint (Int.repr stt))
+    WITH x: Z, stt: Z, v: val, p: val, p1: val, p2: val, r: node_info,
+                    g: gname, gv: globals
+  PRE [ tptr (tptr t_struct_tree), tint, tptr tvoid, tint, tptr tvoid, tptr tvoid]
+  PROP (repable_signed x; is_pointer_or_null v; key_in_range x r.1.2 = true )
+  PARAMS (p; Vint (Int.repr x); v; Vint (Int.repr stt); p1; p2)
   GLOBALS (gv)
-  SEP (mem_mgr gv;
-       (* data_at sh (t_struct_pn) (p, p) b; *)
-       field_at Ews t_struct_tree_t (DOT _t) tp p;
-       field_at Ews t_struct_tree_t (DOT _min) (Vint (Int.repr min)) p;
-       field_at Ews t_struct_tree_t (DOT _max) (Vint (Int.repr max)) p )
+  SEP (mem_mgr gv; node_rep_R nullval r.1.2 r.2 g *
+                     (* (!!(p = r.1.1.1 /\ p = nullval)  && seplog.emp); *)
+       data_at Ews (tptr t_struct_tree) nullval p)
   POST[ tvoid ]
-  EX (pnt : val) (pnl: list val) (lkl: list val),
+  EX (pnt : val),
   PROP (pnt <> nullval)
   LOCAL ()
-  SEP (mem_mgr gv;
-       (* data_at sh t_struct_pn (p, p) b; *)
-       field_at Ews t_struct_tree_t (DOT _t) pnt p;
-       malloc_token Ews t_struct_tree pnt;
-       iter_sepcon (fun pn => malloc_token Ews t_struct_tree_t pn) pnl;
-       iter_sepcon (fun lk => atomic_int_at Ews (vint 0) lk) lkl;
-(*
-       data_at Ews t_struct_tree (vint x, (v, (p1', p2'))) pnt;
-       data_at Ews t_struct_tree_t (Vlong (Int64.repr 0), (lock2, (vint x, vint max))) p2';
-       data_at Ews t_struct_tree_t (Vlong (Int64.repr 0), (lock1, (vint min, vint x))) p1';
-*)
-       field_at Ews t_struct_tree_t (DOT _min) (vint min) p;
-       field_at Ews t_struct_tree_t (DOT _max) (vint max) p).
+  SEP (mem_mgr gv; node_rep_R pnt r.1.2 (Some (Some (x, v, [p1; p2]))) g;
+       data_at Ews (tptr t_struct_tree) pnt p).
 
 Definition Gprog : funspecs :=
     ltac:(with_library prog [acquire_spec; release_spec; makelock_spec;
@@ -159,34 +167,23 @@ Definition Gprog : funspecs :=
 Lemma insertOp: semax_body Vprog Gprog f_insertOp insertOp_spec.
 Proof.
   start_function.
-  forward.
-  forward_call (t_struct_tree_t, gv).
-  Intros p1.
-  forward_call (t_struct_tree_t, gv).
-  Intros p2.
-  forward.
-  assert_PROP (field_compatible t_struct_tree_t [] p1) by entailer!.
-  assert_PROP (field_compatible t_struct_tree_t [] p2) by entailer!.
-  forward. 
-  forward_call (gv).
-  Intros lock1.
-  forward.
-  sep_apply atomic_int_isptr.
-  Intros.
-  forward_call release_nonatomic (lock1).
-  forward_call (gv).
-  Intros lock2.
-  forward.
-  Intros.
-  forward_call release_nonatomic (lock2).
-  (* make lock invariant *)
   forward_call (t_struct_tree, gv).
-  Intros pnt.
-  forward. forward. forward. forward. forward. forward. forward.
-  forward. forward. forward. forward. forward. forward. forward.
-  forward. 
-  Exists pnt [p1; p2] [lock1; lock2].
+  Intros new_node.
+  forward.
+  forward.
+  forward.
+  forward.
+  forward.
+  Exists new_node.
+  assert_PROP (new_node  <> nullval). entailer !.
+  unfold node_rep_R.
+  unfold my_specific_tree_rep.
+
+  rewrite if_false; auto.
+  Search eq_dec.
+  destruct (eq_dec nullval nullval); last first; try easy.
+  Intros. 
   entailer !.
-  simpl.
-  entailer !.
-  Admitted.
+  Exists x v p1 p2.
+  entailer !. 
+Qed.
