concurrency/Modular/implementations/README.md
@@ -1,0 +1,20 @@
+# Run program 
+Running the program for each data structure (linked list or BST) and each template (lock-coupling or giveup template):
+
+``
+make clean 
+make lock list 
+./list
+``
+
+Repeat the process for `bst`, and also for the `giveup` template for both `bst` and `list`.
+
+# Detailed Program
+
+- `data_structure.h` contains interface functions.
+- `bst.c` and `list.c` represent the sequence of BST and list, inheriting from `data_structure.h`.
+- `template.h` and `template.c` are universal files containing `insert` and `lookup` functions.
+- `giveup_template.h` and `giveup_template.c` are files for the giveup template, inheriting from `template.h` and `data_structure.h`.
+- `lock_template.h` and `lock_template.c` are files for the lock-coupling template, inheriting from `template.h` and `data_structure.h`.
+- `bst_giveup.h` and `bst_giveup.c` contain the implementation of `insertOp_giveup`, and `giveup_template.c` will call this function.
+- `bst_lock.h` and `bst_lock.c` contain the implementation of `insertOp_giveup`, and `giveup_template.c` will call this function.
